ZKLib/OracleReduction/Basic.lean
@@ -7,6 +7,8 @@ Authors: Quang Dao
 import VCVio
 import ZKLib.Relation.Basic
 import ZKLib.Data.Math.Fin
+import ZKLib.Data.Math.HList
+import Mathlib.Data.Fin.Fin2
 
 /-!
 # (Interactive) Oracle Reductions
@@ -36,10 +38,14 @@ IOP" [BCG20] (and other kinds of IOPs) from our definition.
 
 -/
 
--- Figure out where to put this instance
-instance instDecidableEqOption {α : Type*} [DecidableEq α] : DecidableEq (Option α) := inferInstance
+set_option linter.docPrime false
 
 open OracleComp OracleSpec SubSpec
+
+section Prelude
+
+-- Figure out where to put this instance
+instance instDecidableEqOption {α : Type*} [DecidableEq α] : DecidableEq (Option α) := inferInstance
 
 /-- `Sampleable` is a type class for types that can be sampled uniformly at random (via the VCV
     framework). This is mostly used for uniform sampling from challenges in an interactive protocol.
@@ -48,6 +54,79 @@ class Sampleable (α : Type) extends Fintype α, Inhabited α, SelectableType α
   [toDecidableEq : DecidableEq α]
 
 instance {α : Type} [Sampleable α] : DecidableEq α := Sampleable.toDecidableEq
+
+/-- Enum type for the direction of a round in a protocol specification -/
+inductive Direction where
+  | P_to_V -- Message
+  | V_to_P -- Challenge
+deriving DecidableEq, Inhabited, Repr
+
+/-- Equivalence between `Direction` and `Fin 2`, sending `V_to_P` to `0` and `P_to_V` to `1`
+(the choice is essentially arbitrary). -/
+def DirectionEquivFin2 : Direction ≃ Fin 2 where
+  toFun := fun dir => match dir with
+    | .V_to_P => ⟨0, by decide⟩
+    | .P_to_V => ⟨1, by decide⟩
+  invFun := fun n => match n with
+    | ⟨0, _⟩ => .V_to_P
+    | ⟨1, _⟩ => .P_to_V
+  left_inv := fun dir => match dir with
+    | .P_to_V => rfl
+    | .V_to_P => rfl
+  right_inv := fun n => match n with
+    | ⟨0, _⟩ => rfl
+    | ⟨1, _⟩ => rfl
+
+/-- This allows us to write `0` for `.V_to_P` and `1` for `.P_to_V`. -/
+instance : Coe (Fin 2) Direction := ⟨DirectionEquivFin2.invFun⟩
+
+end Prelude
+
+section Format
+
+/-- Type signature for an interactive protocol, with `n` messages exchanged. -/
+@[reducible]
+def ProtocolSpec (n : ℕ) := Fin n → Direction × Type
+
+variable {n : ℕ}
+
+abbrev ProtocolSpec.getDir (pSpec : ProtocolSpec n) (i : Fin n) := pSpec i |>.1
+
+abbrev ProtocolSpec.getType (pSpec : ProtocolSpec n) (i : Fin n) := pSpec i |>.2
+
+/-- Subtype of `Fin n` for the indices corresponding to messages in a protocol specification -/
+def MessageIndex (pSpec : ProtocolSpec n) :=
+  {i : Fin n // pSpec.getDir i = Direction.P_to_V}
+
+/-- Subtype of `Fin n` for the indices corresponding to challenges in a protocol specification -/
+def ChallengeIndex (pSpec : ProtocolSpec n) :=
+  {i : Fin n // pSpec.getDir i = Direction.V_to_P}
+
+/-- The type of the `i`-th message in a protocol specification -/
+@[inline, reducible]
+def ProtocolSpec.Message (pSpec : ProtocolSpec n) (i : MessageIndex pSpec) :=
+  pSpec.getType i.val
+
+/-- The type of the `i`-th challenge in a protocol specification -/
+@[inline, reducible]
+def ProtocolSpec.Challenge (pSpec : ProtocolSpec n) (i : ChallengeIndex pSpec) :=
+  pSpec.getType i.val
+
+/-- The transcript of an interactive protocol, which is a list of messages and challenges -/
+@[inline, reducible]
+def Transcript (pSpec : ProtocolSpec n) := (i : Fin n) → pSpec.getType i
+
+variable {ι : Type}
+
+variable {pSpec : ProtocolSpec n} {oSpec : OracleSpec ι} {State : Type}
+
+@[inline, reducible]
+def Transcript.messages (transcript : Transcript pSpec) (i : MessageIndex pSpec) :=
+  transcript i.val
+
+@[inline, reducible]
+def Transcript.challenges (transcript : Transcript pSpec) (i : ChallengeIndex pSpec) :=
+  transcript i.val
 
 /-- `ToOracle` provides an oracle interface for a type `Message`. It defines the query type `Query`,
   the response type `Response`, and the transformation `toOracle` that transforms a message into an
@@ -58,79 +137,54 @@ class ToOracle (Message : Type) where
   Response : Type
   respond : Message → Query → Response
 
-section Format
+-- TODO: Notation for the type signature of an interactive protocol
 
-/-- Type signature of a public-coin interactive protocol.
-`ProtocolSpec` is parameterized by the number of rounds `numRounds`. -/
-@[ext]
-structure ProtocolSpec (numRounds : ℕ) where
-  Message : Fin numRounds → Type -- Message type for each round
-  Challenge : Fin numRounds → Type -- Challenge type for each round
+#eval "𝒫 ——⟦ 𝔽⦃≤ d⦄[X] ⟧⟶ 𝒱"
 
-/-- The empty protocol, with no rounds -/
-@[inline, reducible, simps]
-def emptyPSpec : ProtocolSpec 0 where
-  Message := isEmptyElim
-  Challenge := isEmptyElim
+#eval "𝒫  ⟵⟦ 𝔽 ⟧—— 𝒱"
 
-instance : Inhabited (ProtocolSpec 0) where
-  default := emptyPSpec
+-- TODO: Notation for the objects / elements sent during the protocol
 
-/-- The empty protocol is the unique protocol with 0 rounds -/
-instance : Unique (ProtocolSpec 0) where
-  default := default
-  uniq := fun spec => by ext i <;> exact Fin.elim0 i
+#eval "𝒫  ——[ ∑ x ∈ D ^ᶠ (n - i), peval x (Fin.injOnRight i n) p ]⟶  𝒱"
 
-/-- A protocol with only one round, and with the given message and challenge types -/
-@[inline, reducible, simps]
-def ProtocolSpec.mkSingle (Message : Type) (Challenge : Type) : ProtocolSpec 1 where
-  Message := fun _ => Message
-  Challenge := fun _ => Challenge
-
-variable {n : ℕ} {ι : Type}
+#eval "𝒫  ⟵[ r i ←$ 𝔽 ]—— 𝒱"
 
 /-- Spec for the verifier's challenges, invoked in the process of running the protocol -/
 @[simps]
-def challengeOracle (pSpec : ProtocolSpec n) [∀ i, Sampleable (pSpec.Challenge i)] :
-    OracleSpec (Fin n) where
+def challengeOracle (pSpec : ProtocolSpec n) [S : ∀ i, Sampleable (pSpec.Challenge i)] :
+    OracleSpec (ChallengeIndex pSpec) where
   domain := fun _ => Unit
   range := fun i => pSpec.Challenge i
   domain_decidableEq' := fun _ => decEq
-  range_decidableEq' := fun _ => Sampleable.toDecidableEq
-  range_inhabited' := fun _ => Sampleable.toInhabited
-  range_fintype' := fun _ => Sampleable.toFintype
+  range_decidableEq' := fun i => @Sampleable.toDecidableEq _ (S i)
+  range_inhabited' := fun i => @Sampleable.toInhabited _ (S i)
+  range_fintype' := fun i => @Sampleable.toFintype _ (S i)
 
-/--
-  The transcript of an interactive protocol, which is a list of messages and challenges according to
-  their type signatures.
--/
-@[ext]
-structure Transcript (pSpec : ProtocolSpec n) where
-  messages : ∀ i, pSpec.Message i -- (i : Fin n) → pSpec.Message i
-  challenges : ∀ i, pSpec.Challenge i -- (i : Fin n) → pSpec.Challenge i
 
-@[inline, reducible]
-def emptyTranscript : Transcript emptyPSpec where
-  messages := isEmptyElim
-  challenges := isEmptyElim
+-- Add an indexer?
+structure Indexer (pSpec : ProtocolSpec n) (oSpec : OracleSpec ι) (Index : Type)
+    (Encoding : Type) where
+  encode : Index → OracleComp oSpec Encoding
+  [toOracle : ToOracle Encoding]
+
+-- The prover should be divided into two parts:
+-- Its interaction during the protocol
+-- Its initialization and output
 
 /-- Initialization of prover's state via loading the statement and witness -/
-structure ProverInit (pSpec : ProtocolSpec n) (oSpec : OracleSpec ι) (PrvState : Type)
-    (Statement Witness : Type) where
-  load : Statement → Witness → OracleComp oSpec PrvState
+structure ProverInit (pSpec : ProtocolSpec n) (PrvState : Type) (Statement Witness : Type) where
+  load : Statement → Witness → PrvState
 
-/-- The proving function `prove` for each round of an interactive protocol.
-
-It takes in the round index `i`, the challenge for that round, and performs an oracle
-stateful computation, returning the next message in the protocol.-/
+/-- Represents the interactive prover for a given protocol specification -/
 structure ProverRound (pSpec : ProtocolSpec n) (oSpec : OracleSpec ι) (PrvState : Type) where
-  prove : (i : Fin n) → pSpec.Challenge i →
-    StateT PrvState (OracleComp oSpec) (pSpec.Message i)
+  -- Receive a challenge and update the prover's state
+  receiveChallenge (i : ChallengeIndex pSpec) : PrvState → (pSpec.Challenge i) → PrvState
+  -- Send a message and update the prover's state
+  sendMessage (i : MessageIndex pSpec) : PrvState → OracleComp oSpec (pSpec.Message i × PrvState)
 
-/-- The overall prover of an interactive protocol -/
-class Prover (pSpec : ProtocolSpec n) (oSpec : OracleSpec ι) (PrvState : Type)
-    (Statement Witness : Type) extends ProverRound pSpec oSpec PrvState,
-    ProverInit pSpec oSpec PrvState Statement Witness
+structure Prover (pSpec : ProtocolSpec n) (oSpec : OracleSpec ι) (PrvState : Type)
+    (Statement Witness : Type) extends ProverInit pSpec PrvState Statement Witness,
+    ProverRound pSpec oSpec PrvState
 
 /-- The verifier of an interactive protocol (that may read messages in full) -/
 class Verifier (pSpec : ProtocolSpec n) (oSpec : OracleSpec ι) (Statement : Type) where
@@ -139,22 +193,24 @@ class Verifier (pSpec : ProtocolSpec n) (oSpec : OracleSpec ι) (Statement : Typ
 /-- A list of queries to the prover's messages -/
 @[inline, reducible]
 def QueryList (pSpec : ProtocolSpec n) [O : ∀ i, ToOracle (pSpec.Message i)] :=
-  List ((i : Fin n) × (O i).Query)
+  List ((i : MessageIndex pSpec) × (O i).Query)
 
 /-- A list of responses to queries, computed from the prover's messages -/
 @[inline, reducible]
 def ResponseList (pSpec : ProtocolSpec n) [O : ∀ i, ToOracle (pSpec.Message i)] :=
-  List ((i : Fin n) × (O i).Query × (O i).Response)
+  List ((i : MessageIndex pSpec) × (O i).Query × (O i).Response)
 
 /-- The verifier of an interactive oracle protocol
 (that may only make queries to the prover's messages) -/
-structure OracleVerifier (pSpec : ProtocolSpec n) [O : ∀ i, ToOracle (pSpec.Message i)]
-    (oSpec : OracleSpec ι) (Statement : Type) where
+structure OracleVerifier (pSpec : ProtocolSpec n) (oSpec : OracleSpec ι)
+    [O : ∀ i, ToOracle (pSpec.Message i)] (Statement : Type) where
   -- Generate a list of queries of the form `(i, query)`,
   -- where `i` is the round index and `query` is the query to the oracle
-  genQueries : Statement → (∀ i, pSpec.Challenge i) → OracleComp oSpec (QueryList pSpec)
+  genQueries : Statement → (∀ i, pSpec.Challenge i) →
+      OracleComp oSpec (QueryList pSpec)
   -- Verify the proof based on the list of responses
-  verify : Statement → (∀ i, pSpec.Challenge i) → ResponseList pSpec → OracleComp oSpec Bool
+  verify : Statement → (∀ i, pSpec.Challenge i) → ResponseList pSpec →
+      OracleComp oSpec Bool
 
 /-- We can always turn an oracle verifier into a (non-oracle) verifier -/
 def OracleVerifier.toVerifier {pSpec : ProtocolSpec n} {oSpec : OracleSpec ι} {Statement : Type}
@@ -199,130 +255,110 @@ section Restrict
 
 variable {n : ℕ}
 
-/-- For a protocol specification `pSpec` with `n` rounds, restrict `pSpec` to the first `cutoff`
-  rounds. -/
-@[inline, reducible, simps]
-def ProtocolSpec.take (pSpec : ProtocolSpec n) (cutoff : ℕ) (h : cutoff ≤ n) :
-    ProtocolSpec cutoff where
-  Message := Fin.take pSpec.Message cutoff h
-  Challenge := Fin.take pSpec.Challenge cutoff h
+abbrev ProtocolSpec.take (m : ℕ) (h : m ≤ n) (pSpec : ProtocolSpec n) :=
+  Fin.take m h pSpec
 
-/-- For a protocol specification `pSpec` with `n` rounds, restrict `pSpec` to the last `cutoff`
-  rounds. -/
-@[inline, reducible, simps]
-def ProtocolSpec.rtake (pSpec : ProtocolSpec n) (cutoff : ℕ) (h : cutoff ≤ n) :
-    ProtocolSpec cutoff where
-  Message := Fin.rtake pSpec.Message cutoff h
-  Challenge := Fin.rtake pSpec.Challenge cutoff h
+abbrev ProtocolSpec.rtake (m : ℕ) (h : m ≤ n) (pSpec : ProtocolSpec n) :=
+  Fin.rtake m h pSpec
 
-@[simp]
-theorem ProtocolSpec.take_nil (pSpec : ProtocolSpec n) :
-    ProtocolSpec.take pSpec 0 (by omega) = default := by
-  ext i <;> exact Fin.elim0 i
+abbrev Transcript.take {pSpec : ProtocolSpec n} (m : ℕ) (h : m ≤ n)
+    (transcript : Transcript pSpec) : Transcript (pSpec.take m h) :=
+  Fin.take m h transcript
 
-@[simp]
-theorem ProtocolSpec.take_self (pSpec : ProtocolSpec n) :
-    ProtocolSpec.take pSpec n (by omega) = pSpec := by
-  ext i <;> simp [ProtocolSpec.take]
-
-@[simp]
-theorem ProtocolSpec.rtake_nil (pSpec : ProtocolSpec n) :
-    ProtocolSpec.rtake pSpec 0 (by omega) = default := by
-  ext i <;> exact Fin.elim0 i
-
-@[simp]
-theorem ProtocolSpec.rtake_self (pSpec : ProtocolSpec n) :
-    ProtocolSpec.rtake pSpec n (by omega) = pSpec := by
-  ext i <;> simp [ProtocolSpec.rtake, Fin.natAdd]
-
-def Transcript.take {pSpec : ProtocolSpec n} (cutoff : ℕ) (h : cutoff ≤ n)
-    (transcript : Transcript pSpec) : Transcript (pSpec.take cutoff h) where
-  messages := Fin.take transcript.messages cutoff h
-  challenges := Fin.take transcript.challenges cutoff h
-
-def Transcript.rtake {pSpec : ProtocolSpec n} (cutoff : ℕ) (h : cutoff ≤ n)
-    (transcript : Transcript pSpec) : Transcript (pSpec.rtake cutoff h) where
-  messages := Fin.rtake transcript.messages cutoff h
-  challenges := Fin.rtake transcript.challenges cutoff h
+abbrev Transcript.rtake {pSpec : ProtocolSpec n} (m : ℕ) (h : m ≤ n)
+    (transcript : Transcript pSpec) : Transcript (pSpec.rtake m h) :=
+  Fin.rtake m h transcript
 
 end Restrict
 
 section Composition
 
-variable {m n : ℕ}
+variable {n m : ℕ}
 
-/-- Adding a round with type `Message` and `Challenge` to the beginning of a `ProtocolSpec` -/
-def ProtocolSpec.cons (pSpec : ProtocolSpec n) (Message : Type) (Challenge : Type) :
-    ProtocolSpec (n + 1) where
-  Message := Fin.cons Message pSpec.Message
-  Challenge := Fin.cons Challenge pSpec.Challenge
+/-- Adding a round with direction `dir` and type `Message` to the beginning of a `ProtocolSpec` -/
+abbrev ProtocolSpec.cons (pSpec : ProtocolSpec n) (dir : Direction) (Message : Type) :
+    ProtocolSpec (n + 1) :=
+  Fin.cons ⟨dir, Message⟩ pSpec
 
-/-- Adding a round with type `Message` and `Challenge` to the end of a `ProtocolSpec` -/
-def ProtocolSpec.snoc (pSpec : ProtocolSpec n) (Message : Type) (Challenge : Type) :
-    ProtocolSpec (n + 1) where
-  Message := Fin.snoc pSpec.Message Message
-  Challenge := Fin.snoc pSpec.Challenge Challenge
+/-- Adding a round with direction `dir` and type `Message` to the end of a `ProtocolSpec` -/
+abbrev ProtocolSpec.snoc (pSpec : ProtocolSpec n) (dir : Direction) (Message : Type) :
+    ProtocolSpec (n + 1) :=
+  Fin.snoc pSpec ⟨dir, Message⟩
 
-/-- Appending two `ProtocolSpec`s via appending their `Message` and `Challenge` types -/
-def ProtocolSpec.append (pSpec : ProtocolSpec m) (pSpec' : ProtocolSpec n) :
-    ProtocolSpec (m + n) where
-  Message := Fin.append pSpec.Message pSpec'.Message
-  Challenge := Fin.append pSpec.Challenge pSpec'.Challenge
+/-- Appending two `ProtocolSpec`s -/
+abbrev ProtocolSpec.append (pSpec : ProtocolSpec n) (pSpec' : ProtocolSpec m) :
+    ProtocolSpec (n + m) :=
+  Fin.append pSpec pSpec'
+
+def ProtocolSpec.mkSingle (dir : Direction) (Message : Type) : ProtocolSpec 1 :=
+  fun _ => ⟨dir, Message⟩
 
 infixl : 65 " ++ₚ " => ProtocolSpec.append
 
 @[simp]
-theorem ProtocolSpec.snoc_eq_append {Message Challenge : Type} {pSpec : ProtocolSpec m} :
-    pSpec.snoc Message Challenge = pSpec ++ₚ .mkSingle Message Challenge := by
-  ext i <;> simp [ProtocolSpec.append, ProtocolSpec.snoc, Fin.snoc_eq_append] <;>
-  congr <;> unfold Fin.cons <;> ext j
-  · have h : j = 0 := by aesop
-    subst h ; simp
-  · have h : j = 0 := by aesop
-    subst h ; simp
-
-@[simp]
-theorem ProtocolSpec.append_take {pSpec : ProtocolSpec n} (m : Fin n) :
-    (pSpec.take m (by omega) ++ₚ .mkSingle (pSpec.Message m) (pSpec.Challenge m))
+theorem ProtocolSpec.snoc_take {pSpec : ProtocolSpec n} (m : ℕ) (h : m < n) :
+    (pSpec.take m (by omega) ++ₚ (fun (_ : Fin 1) => pSpec ⟨m, h⟩))
         = pSpec.take (m + 1) (by omega) := by
-  ext i <;> simp only [append] <;> rw [Fin.take_succ_eq_snoc] <;>
-  simp [Fin.snoc_eq_append] <;> congr <;> unfold Fin.cons <;> ext j
-  · have : j = 0 := by aesop
-    subst this ; simp
-  · have : j = 0 := by aesop
-    subst this ; simp
+  simp only [append, take, Fin.append_right_eq_snoc, Fin.take_succ_eq_snoc]
 
 /-- Appending two `ToOracle`s for two `ProtocolSpec`s -/
-def ToOracle.append {pSpec : ProtocolSpec m} {pSpec' : ProtocolSpec n}
-    [O : ∀ i, ToOracle (pSpec.Message i)] [O' : ∀ i, ToOracle (pSpec'.Message i)] :
-        ∀ i, ToOracle ((pSpec ++ₚ pSpec').Message i) :=
-  Fin.addCases_fun O O'
+def ToOracle.append {pSpec₁ : ProtocolSpec n} {pSpec₂ : ProtocolSpec m}
+    [O₁ : ∀ i, ToOracle (pSpec₁.Message i)] [O₂ : ∀ i, ToOracle (pSpec₂.Message i)] :
+        ∀ i, ToOracle ((pSpec₁ ++ₚ pSpec₂).Message i) := fun ⟨i, h⟩ => by
+  dsimp [ProtocolSpec.append, ProtocolSpec.getDir] at h ⊢
+  dsimp [ProtocolSpec.Message, ProtocolSpec.getType]
+  by_cases h' : i < n
+  · rw [← Fin.castAdd_castLT m i h', Fin.append_left] at h ⊢
+    exact O₁ ⟨i.castLT h', h⟩
+  · rw [← @Fin.natAdd_subNat_cast n m i (not_lt.mp h'), Fin.append_right] at h ⊢
+    exact O₂ ⟨Fin.subNat n (Fin.cast (add_comm n m) i) (not_lt.mp h'), h⟩
 
 /-- Appending two transcripts for two `ProtocolSpec`s -/
-def Transcript.append {pSpec : ProtocolSpec m} {pSpec' : ProtocolSpec n}
-    (T : Transcript pSpec) (T' : Transcript pSpec') : Transcript (pSpec ++ₚ pSpec') where
-  messages := Fin.addCases' T.messages T'.messages
-  challenges := Fin.addCases' T.challenges T'.challenges
+def Transcript.append {pSpec₁ : ProtocolSpec n} {pSpec₂ : ProtocolSpec m}
+    (T₁ : Transcript pSpec₁) (T₂ : Transcript pSpec₂) : Transcript (pSpec₁ ++ₚ pSpec₂) := by
+  dsimp [ProtocolSpec.append, ProtocolSpec.getDir]
+  dsimp [Transcript, ProtocolSpec.getType] at T₁ T₂ ⊢
+  exact fun i => (Fin.append_comp Prod.snd i) ▸ (Fin.addCases' T₁ T₂ i)
 
-/-- Adding a message and challenge to the end of a `Transcript` -/
-def Transcript.snoc {pSpec : ProtocolSpec n} {NextMessage NextChallenge : Type}
-    (T : Transcript pSpec) (msg : NextMessage) (challenge : NextChallenge) :
-        Transcript (pSpec ++ₚ .mkSingle NextMessage NextChallenge) :=
-  Transcript.append T ⟨fun _ => msg, fun _ => challenge⟩
+infixl : 65 " ++ₜ " => Transcript.append
+
+/-- Adding a message with a given direction and type to the end of a `Transcript` -/
+def Transcript.snoc {pSpec : ProtocolSpec n} {NextMessage : Type}
+    (T : Transcript pSpec) (dir : Direction) (msg : NextMessage) :
+        Transcript (pSpec ++ₚ .mkSingle dir NextMessage) :=
+  Transcript.append T fun _ => msg
 
 end Composition
 
 section Execution
 
-variable {n : ℕ} {pSpec : ProtocolSpec n} {ι : Type} [DecidableEq ι] {oSpec : OracleSpec ι}
+variable {n : ℕ} {pSpec : ProtocolSpec n} {ι : Type} {oSpec : OracleSpec ι}
 {PrvState : Type} {Statement Witness : Type}
+
+/-- Run the prover in the interactive protocol. Returns the final prover's state.
+TODO: Return the transcript as well -/
+def Prover.run (prover : Prover pSpec oSpec PrvState Statement Witness)
+    (chals : ∀ i, pSpec.Challenge i) (state : PrvState) :
+        OracleComp oSpec PrvState :=
+  let rec loop (i : ℕ) (state : PrvState) (chals : ∀ i, pSpec.Challenge i) :
+      OracleComp oSpec PrvState :=
+    if h : i < n then
+      letI i' : Fin n := ⟨i, h⟩
+      match hDir : pSpec.getDir i' with
+      | .V_to_P => loop (i + 1) (prover.receiveChallenge ⟨i', hDir⟩ state (chals ⟨i', hDir⟩)) chals
+      | .P_to_V => do
+        let ⟨ msg, state' ⟩ ← prover.sendMessage ⟨i', hDir⟩ state
+        loop (i + 1) state' chals
+    else
+      pure state
+  loop 0 state chals
 
 /--
   Auxiliary function for running the prover in an interactive protocol. Given round index `i`,
   returns the transcript up to that round, the log of oracle queries made by the prover to `oSpec`
   up to that round, and the prover's state after that round.
 -/
-def runProverAux [∀ i, Sampleable (pSpec.Challenge i)]
+def runProverAux [DecidableEq ι] [∀ i, Sampleable (pSpec.Challenge i)]
     (prover : Prover pSpec oSpec PrvState Statement Witness)
     (stmt : Statement) (wit : Witness) (i : Fin (n + 1)) :
       OracleComp (oSpec ++ₒ challengeOracle pSpec)
@@ -330,25 +366,38 @@ def runProverAux [∀ i, Sampleable (pSpec.Challenge i)]
   induction i using Fin.induction with
   | zero => simp; exact
     (do
-      let ⟨state, queryLog⟩ ← liftComp (simulate loggingOracle ∅ (prover.load stmt wit))
-      return ⟨emptyTranscript, queryLog, state⟩)
-  | succ j ih => simp at ih ⊢; exact
+      let ⟨state, queryLog⟩ ← liftComp (simulate loggingOracle ∅ <| pure (prover.load stmt wit))
+      return ⟨fun i => Fin.elim0 i, queryLog, state⟩)
+  | succ j ih => simp [ProtocolSpec.take] at ih ⊢; exact
     (do
       let ⟨transcript, queryLog, state⟩ ← ih
-      let challenge : pSpec.Challenge j ← query (Sum.inr j) ()
-      let ⟨⟨msg, newState⟩, newQueryLog⟩ ← liftComp
-        (simulate loggingOracle queryLog ((prover.prove j challenge) state))
-      let newTranscript := transcript.snoc msg challenge
-      let newTranscript : Transcript (pSpec.take (j + 1) (by omega)) := by
-        simp only [ProtocolSpec.append_take] at newTranscript
-        exact newTranscript
-      return ⟨newTranscript, newQueryLog, newState⟩)
+      match hDir : pSpec.getDir j with
+      | .V_to_P => do
+        let challenge ← query (Sum.inr ⟨j, hDir⟩) ()
+        haveI challenge : pSpec.Challenge ⟨j, hDir⟩ := by simpa only
+        let newState := prover.receiveChallenge ⟨j, hDir⟩ state challenge
+        let newTranscript := transcript.snoc .V_to_P challenge
+        let newTranscript : Transcript (pSpec.take (j + 1) (by omega)) := by
+          sorry
+          -- simp [ProtocolSpec.snoc_take] at newTranscript
+          -- exact newTranscript
+        return ⟨newTranscript, queryLog, newState⟩
+      | .P_to_V => do
+        let ⟨⟨msg, newState⟩, newQueryLog⟩ ← liftComp
+          (simulate loggingOracle queryLog (prover.sendMessage ⟨j, hDir⟩ state))
+        let newTranscript := transcript.snoc .P_to_V msg
+        let newTranscript : Transcript (pSpec.take (j + 1) (by omega)) := by
+          sorry
+          -- simp only [ProtocolSpec.snoc_take] at newTranscript
+          -- exact newTranscript
+        return ⟨newTranscript, newQueryLog, newState⟩
+      )
 
 /--
   Run the prover in the interactive protocol. Returns the transcript along with the final prover's
   state
 -/
-def runProver [∀ i, Sampleable (pSpec.Challenge i)]
+def runProver [DecidableEq ι] [∀ i, Sampleable (pSpec.Challenge i)]
     (prover : Prover pSpec oSpec PrvState Statement Witness)
     (stmt : Statement) (wit : Witness) : OracleComp
     (oSpec ++ₒ challengeOracle pSpec)
@@ -377,7 +426,6 @@ def runOracleVerifier [O : ∀ i, ToOracle (pSpec.Message i)]
   let decision ← verifier.verify stmt transcript.challenges responses
   return ⟨decision, responses⟩
 
-omit [DecidableEq ι] in
 /-- Running an oracle verifier then discarding the query list is equivalent to
 running a non-oracle verifier -/
 @[simp]
@@ -395,7 +443,7 @@ theorem runOracleVerifier_eq_runVerifier [∀ i, ToOracle (pSpec.Message i)]
   Returns the verifier's decision, the protocol transcript, the log of prover's queries to `oSpec`,
   and the prover's final state
 -/
-def runProtocol [∀ i, Sampleable (pSpec.Challenge i)]
+def runProtocol [DecidableEq ι] [∀ i, Sampleable (pSpec.Challenge i)]
 (protocol : Protocol pSpec oSpec PrvState Statement Witness)
     (stmt : Statement) (wit : Witness) : OracleComp
     (oSpec ++ₒ challengeOracle pSpec)
@@ -412,7 +460,7 @@ to the prover's messages, the log of all prover's queries to `oSpec`, and the pr
 Note: we put `ResponseList pSpec` first so that the rest can be `Prod.snd`, which
 we will show is the same result as doing `runProtocol`.
 -/
-def runOracleProtocol [∀ i, Sampleable (pSpec.Challenge i)]
+def runOracleProtocol [DecidableEq ι] [∀ i, Sampleable (pSpec.Challenge i)]
     [∀ i, ToOracle (pSpec.Message i)]
     (protocol : OracleProtocol pSpec oSpec PrvState Statement Witness)
     (stmt : Statement) (wit : Witness) : OracleComp
@@ -426,7 +474,7 @@ def runOracleProtocol [∀ i, Sampleable (pSpec.Challenge i)]
 /-- Running an oracle verifier then discarding the query list is equivalent to
 running a non-oracle verifier -/
 @[simp]
-theorem runOracleProtocol_eq_runProtocol [∀ i, Sampleable (pSpec.Challenge i)]
+theorem runOracleProtocol_eq_runProtocol [DecidableEq ι] [∀ i, Sampleable (pSpec.Challenge i)]
     [∀ i, ToOracle (pSpec.Message i)]
     (protocol : OracleProtocol pSpec oSpec PrvState Statement Witness)
     (stmt : Statement) (wit : Witness) :
