ZKLib/OracleReduction/Composition.lean
@@ -17,75 +17,96 @@ import ZKLib.Data.Math.Fin
 
 section Composition
 
-variable {n m : ℕ} {PSpec : ProtocolSpec n} {PSpec' : ProtocolSpec m} {ι : Type} [DecidableEq ι]
-    {OSpec : OracleSpec ι} {PrvState Statement Witness : Type}
+variable {n m : ℕ} {pSpec : ProtocolSpec n} {pSpec' : ProtocolSpec m} {ι : Type} [DecidableEq ι]
+    {oSpec : OracleSpec ι} {PrvState Statement Witness : Type}
 
 @[simp]
-theorem ProtocolSpec.take_append_eq_self (PSpec : ProtocolSpec n) (PSpec' : ProtocolSpec m) :
-    (PSpec ++ₚ PSpec').take n (by omega) = PSpec := by
-  simp [ProtocolSpec.append, ProtocolSpec.take]
+theorem ProtocolSpec.take_append_left :
+    (pSpec ++ₚ pSpec').take n (Nat.le_add_right n m) = pSpec := by
+  simp only [take, append]
+  have {i : Fin n} : Fin.castLE (by omega) i = Fin.castAdd m i := by
+    simp only [Fin.castLE, Fin.castAdd]
+  ext i <;>
+  simp only [Fin.take_apply, this, Fin.append_left]
 
-def ProverRound.append (P : ProverRound PSpec OSpec PrvState)
-  (P' : ProverRound PSpec' OSpec PrvState) :
-  ProverRound (PSpec ++ₚ PSpec') OSpec PrvState where
-  prove := fun i => by
-    refine Fin.addCases ?_ ?_ i <;> intro j c <;>
-    simp [ProtocolSpec.append] at c ⊢
-    · exact P.prove j c
-    · exact P'.prove j c
+@[simp]
+theorem Transcript.take_append_left (T : Transcript pSpec) (T' : Transcript pSpec') :
+    ((T ++ₜ T').take n (Nat.le_add_right n m)) =
+      (@ProtocolSpec.take_append_left _ _ pSpec pSpec').symm ▸ T := by
+  simp [Transcript.append, Transcript.take]
+  have {i : Fin n} : Fin.castLE (by omega) i = Fin.castAdd m i := by
+    simp [Fin.castLE, Fin.castAdd]
+  simp [eqRec_eq_cast]
+  ext i
+  simp [Fin.take_apply, Fin.castLE, Fin.addCases', Fin.addCases]
+  sorry
 
-def Prover.append (P : Prover PSpec OSpec PrvState Statement Witness)
-    (P' : ProverRound PSpec' OSpec PrvState) :
-        Prover (PSpec ++ₚ PSpec') OSpec PrvState Statement Witness where
+def ProverRound.append (P : ProverRound pSpec oSpec PrvState)
+  (P' : ProverRound pSpec' oSpec PrvState) :
+  ProverRound (pSpec ++ₚ pSpec') oSpec PrvState := sorry
+  -- receiveChallenge := fun ⟨i, h⟩ => by
+  --   refine Fin.addCases ?_ ?_ i <;> intro j c <;>
+  --   simp [ProtocolSpec.append] at c ⊢
+  --   · exact P.receiveChallenge j c
+  --   · exact P'.receiveChallenge j c
+  -- sendMessage := fun ⟨i, h⟩ => by
+  --   refine Fin.addCases ?_ ?_ i <;> intro j c <;>
+  --   simp [ProtocolSpec.append] at c ⊢
+  --   · exact P.sendMessage j c
+  --   · exact P'.sendMessage j c
+
+def Prover.append (P : Prover pSpec oSpec PrvState Statement Witness)
+    (P' : ProverRound pSpec' oSpec PrvState) :
+        Prover (pSpec ++ₚ pSpec') oSpec PrvState Statement Witness where
   load := P.load
   toProverRound := ProverRound.append P.toProverRound P'
 
 /-- Composition of verifiers. Return the conjunction of the decisions of the two verifiers. -/
-def Verifier.append (V : Verifier PSpec OSpec Statement) (V' : Verifier PSpec' OSpec Statement) :
-    Verifier (PSpec ++ₚ PSpec') OSpec Statement where
+def Verifier.append (V : Verifier pSpec oSpec Statement) (V' : Verifier pSpec' oSpec Statement) :
+    Verifier (pSpec ++ₚ pSpec') oSpec Statement where
   verify := fun stmt transcript => do
-    let firstTranscript : Transcript PSpec := by
+    let firstTranscript : Transcript pSpec := by
       have := transcript.take n (by omega)
       simp at this; exact this
     let decision ← V.verify stmt firstTranscript
-    let secondTranscript : Transcript PSpec' := by
+    let secondTranscript : Transcript pSpec' := by
       have := transcript.rtake m (by omega)
       sorry
     let decision' ← V'.verify stmt secondTranscript
     return decision ∧ decision'
 
-def Protocol.append (P : Protocol PSpec OSpec PrvState Statement Witness)
-    (P' : Protocol PSpec' OSpec PrvState Statement Witness) :
-    Protocol (PSpec ++ₚ PSpec') OSpec PrvState Statement Witness := sorry
+def Protocol.append (P : Protocol pSpec oSpec PrvState Statement Witness)
+    (P' : Protocol pSpec' oSpec PrvState Statement Witness) :
+    Protocol (pSpec ++ₚ pSpec') oSpec PrvState Statement Witness := sorry
   -- prover := Prover.append P.prover P'.prover
   -- verifier := Verifier.append P.verifier P'.verifier
 
-instance [O : ∀ i, ToOracle (PSpec.Message i)] [O' : ∀ i, ToOracle (PSpec'.Message i)] :
-    ∀ i, ToOracle ((PSpec ++ₚ PSpec').Message i) := fun i =>
-  {
-    Query := Fin.addCases (fun j => (O j).Query) (fun j => (O' j).Query) i
-    Response := Fin.addCases (fun j => (O j).Response) (fun j => (O' j).Response) i
-    respond := fun msg query => by sorry
-  }
+instance [O : ∀ i, ToOracle (pSpec.Message i)] [O' : ∀ i, ToOracle (pSpec'.Message i)] :
+    ∀ i, ToOracle ((pSpec ++ₚ pSpec').Message i) := sorry
+  -- {
+  --   Query := Fin.addCases (fun j => (O j).Query) (fun j => (O' j).Query) i
+  --   Response := Fin.addCases (fun j => (O j).Response) (fun j => (O' j).Response) i
+  --   respond := fun msg query => by sorry
+  -- }
     -- refine Fin.addCases ?_ ?_ i <;> intro j c <;>
     --   simp [ProtocolSpec.append] at c ⊢
     --   · exact (O j).respond (fun j => (O j).Query) (fun j => (O j).Response) query response
     --   · exact (O' j).respond (fun j => (O' j).Query) (fun j => (O' j).Response) query response
 
-def OracleVerifier.append [O : ∀ i, ToOracle (PSpec.Message i)]
-    [O' : ∀ i, ToOracle (PSpec'.Message i)] (V : OracleVerifier PSpec OSpec Statement)
-    (V' : OracleVerifier PSpec' OSpec Statement) :
-        OracleVerifier (PSpec ++ₚ PSpec') OSpec Statement := sorry
+def OracleVerifier.append [O : ∀ i, ToOracle (pSpec.Message i)]
+    [O' : ∀ i, ToOracle (pSpec'.Message i)] (V : OracleVerifier pSpec oSpec Statement)
+    (V' : OracleVerifier pSpec' oSpec Statement) :
+        OracleVerifier (pSpec ++ₚ pSpec') oSpec Statement := sorry
   -- genQueries := fun stmt transcript => do
   --   let queries ← V.genQueries stmt transcript.challenges
   --   let queries' ← V'.genQueries stmt transcript.challenges
   --   return queries ++ queries'
   -- verify := fun stmt transcript responseList => do
-  --   let firstTranscript : Transcript PSpec := by
+  --   let firstTranscript : Transcript pSpec := by
   --     have := transcript.take n (by omega)
   --     simp at this; exact this
   --   let decision ← V.verify stmt firstTranscript
-  --   let secondTranscript : Transcript PSpec' := by
+  --   let secondTranscript : Transcript pSpec' := by
   --     have := transcript.rtake m (by omega)
   --     sorry
   --   let decision' ← V'.verify stmt secondTranscript
@@ -93,11 +114,9 @@ def OracleVerifier.append [O : ∀ i, ToOracle (PSpec.Message i)]
 
 -- Define composition of multiple protocols via recursion
 
-def ProtocolSpec.appendMany (rounds : List ℕ)
-    (PSpecs : ∀ i : Fin rounds.length, ProtocolSpec (rounds.get i)) :
-    ProtocolSpec (List.sum rounds) where
-  Message := sorry
-  Challenge := sorry
+def ProtocolSpec.appendList (rounds : List ℕ)
+    (pSpecs : ∀ i : Fin rounds.length, ProtocolSpec (rounds.get i)) :
+    ProtocolSpec rounds.sum := sorry
 
 end Composition
 
